# Note 23 - April 4

# Review

$$
\begin{aligned}
&\text{Birth rates: }\lambda_i = R_{i,i+1}\quad\quad i=0,1,\cdots\\
&\text{Death rates: }\mu_i = R_{i,i-1}\quad\quad i=1,2,\cdots
\end{aligned}\\

R=\begin{pmatrix}
    -\lambda_0 & \lambda_0   \\
    \mu_1&-(\lambda_1+\mu_1)&\lambda_1 \\
    & \mu_2&-(\lambda_2+\mu_2)&\lambda_2 \\
    &&\mu_3&-(\lambda_3+\mu_3)&\lambda_3 \\\\
    &&\quad\quad\quad\ddots&\quad\quad\quad\ddots&\quad\quad\quad\ddots
\end{pmatrix}\\
\Rightarrow
\begin{aligned}
    &R_{ii} =-(\lambda_i+\mu_i) \quad i\geq 1    \\
    &R_{00} =\lambda_0
\end{aligned}
$$


# 6. Continuous-Time Markov Chain (cont'd)

## 6.5. Birth and Death Processes (cont'd)

As we see, there are two main types of birth and death processes: __queueing system__ and __population model__. THe key difference between them is that the birth rate in the queueing system is typically a constant (does not depend on the current state $i$), while the birth rate in population model increases as $i$ increases.

### 6.5.1. Stationary Distribution of a Birth and Death Process

$$ \begin{cases}
    \underline{\pi}\cdot R = \underline{0}\quad (1)\\
    \underline{\pi}\cdot 1\!\!\!\!\perp = \underline1 \quad (2)\\
\end{cases} $$

$$
(\pi_0,\pi_1,\cdots) \cdot \begin{pmatrix}
    -\lambda_0 & \lambda_0 \\
    \mu_1 & -(\lambda_1+\mu_1)&\lambda_1\\
    &\mu_2 & -(\lambda_2+\mu_2)&\lambda_2\\\\
    && \quad\quad\ddots& \quad\quad\ddots& \quad\quad\ddots
\end{pmatrix}
$$

$$ (1) \Rightarrow
\begin{aligned}
&-\lambda_0\pi_0+\mu_1\pi_1 = 0 \Rightarrow\pi_1=\frac{\lambda_0}{\mu_1}\pi_0\\
&\lambda_0\pi_0-(\lambda_1+\mu_1)\mu_1+\mu_2\pi_2 = 0
    
\end{aligned}
$$
Add this to the first equation, we have
$$ -\lambda_1\pi_1+\mu_2\pi_2 = 0 \Rightarrow\pi_2=\frac{\lambda_1}{\mu_2}\pi_1 $$

In general, adding the first $i$ equations, we have
$$ -\lambda_0\pi_0+\mu_1\pi_1= 0 $$
$$ \lambda_0\pi_0-(\lambda_1+\mu_1)\pi_1+\mu_2\pi_2=0 $$
$$ \vdots $$
$$ \lambda_{i-2}\pi_{i-2}-(\lambda_{i-1}+\mu_{i-1}+\mu_i\pi_i)=0 $$
$$ -\lambda_{i-1}\pi_{i-1}+\mu_i\pi_i=0 $$
$$ \begin{aligned}
    \Rightarrow \pi_i &= \frac{\lambda_{i-1}}{\mu_i}\pi_{i-1}\\
    &=\cdots\\
    &=\frac{\lambda_0\lambda_1\cdots\lambda_{i-1}}{\mu_1\mu_2\cdots\mu_i}\pi_0
\end{aligned} $$

Use $(2)$ to normalize
$$ 1=\sum_{n=0}^\infty \pi_n = (1+\sum_{n=1}^{\infty}\Pi_{j=1}^n\frac{\lambda_{j-1}}{\mu_j} $$
$$ 
\begin{aligned}
\Rightarrow
&\pi_0=\frac{1}{1+\sum_{n=1}^\infty\Pi_{j=1}^n\frac{\lambda_{j-1}}{\mu_j}}\\
&\pi_i=\frac{\Pi_{j=1}^i\frac{\lambda_{j-1}}{\mu_j}}{1+\sum_{n=1}^\infty\Pi_{j=1}^n\frac{\lambda_{j-1}}{\mu_j}}
\end{aligned}
$$

Thus, a stationary distribution exists(the MC is positive recurrent, assuming irreducible) if and only if
$$ \sum_{n=1}^\infty\Pi_{j=1}^n\frac{\lambda_{j-1}}{\mu_j } < \infty $$

#### Example 6.5.1.1. M/M/S Queue (cont'd)

$$ \lambda_i = \lambda\quad\quad\mu_i=\begin{cases}
    i\mu\quad i\leq s \\
    s\mu\quad i>s
\end{cases} $$

$$
\begin{aligned}
&\sum_{n=1}^\infty \Pi_{j=1}^n\frac{\lambda_{j-1}}{\mu_j}\\
&= \underbrace{\frac{\lambda}{\mu}+\frac{\lambda}{\mu}\cdot\frac{\lambda}{2\mu}+\cdots+\frac{\lambda}{\mu}\frac{\lambda}{2\mu}\cdots\frac{\lambda}{s\mu} + \frac{\lambda}{\mu}\frac{\lambda}{2\mu}\cdots(\frac{\lambda}{s\mu})^2+\frac{\lambda}{\mu}\frac{\lambda}{2\mu}\cdots(\frac{\lambda}{s\mu})^3+\cdots}_{\text{geometric series with ration $\frac{\lambda}{s\mu}$}}
\end{aligned}
$$

$\Rightarrow$ The sum is finite if and only if $\lambda<s\mu$

$\Rightarrow$ the process $\{X(t)\}_{t\geq 0}$ is positive recurrent if and only if $\underbrace{\lambda}_{\text{arrival rate}} < \underbrace{s\mu}_{\text{maximal (total) service rate}}$

#### Example 6.5.1.2. Population Model (with immigration)

$$ \lambda_i=i\lambda+\alpha\quad\quad\mu_i=i\mu $$

$$
\sum_{n=1}^\infty \Pi_{j=1}^n\frac{\lambda_{j-1}}{\mu_j} = \sum_{n=1}^\infty\Pi_{j=1}^n\frac{(j-1)\lambda+\alpha}{j\mu}
$$
$$
\lim_{j\rightarrow\infty}\frac{(j-1)\lambda+\alpha}{j\mu}=\frac{\lambda}{\mu}
$$
If $\lambda<\mu$, then $\quad\sum_{n=1}^\infty\Pi_{j=1}^n\frac{(j-1)\lambda+\alpha}{j\mu}<\infty$ by ratio test.

If $\lambda>\mu$, then $\quad\sum_{n=1}^\infty\Pi_{j=1}^n\frac{(j-1)\lambda+\alpha}{j\mu}=\infty$.

If $\lambda=\mu$, then $\quad\alpha \geq \lambda =\mu$, the ratio $\frac{(j-1)\lambda+\alpha}{j\mu}\geq 1$ for all $j$

$\Rightarrow$ the terms in the summation is non-decreasing

$\Rightarrow$ the $sum = \infty$

If $\lambda=\mu,\quad \alpha <\lambda = \mu$ï¼š

__Raabe-Duhamel's test__: (not required content)
$$ L:=\lim_{n\rightarrow\infty} n(\frac{a_n}{a_{n+1}}-1)\begin{cases}
    >1\quad\text{converge}\\
    <1\quad\text{diverge}\\
    =1\quad\text{inconclusive}\\
\end{cases} $$

Here:
$$
\begin{aligned}
L&=\lim_{n\rightarrow\infty}n(\frac{n\mu}{(n-1)\lambda+\alpha})\\
&=\lim_{n\rightarrow\infty}n(\frac{n\lambda-(n-1)\lambda-\alpha}{(n-1)\lambda+\alpha})\\
&=\lim_{n\rightarrow\infty}n(\frac{\lambda-\alpha}{(n-1)\lambda+\alpha})\\
&=\frac{\lambda-\alpha}{\lambda} <1
\end{aligned}
$$
$\Rightarrow$ the sum $=\infty$

##### Conclusion

To sum up, the CTMC is positive recurrent if and only if $\lambda<\mu$

__Q__: What happens if $\lambda_0=0$? (0 is absorbing)

__A__:

The chain is not irreducible; typically two classes:

- $\{0\}\quad\quad\quad\quad\quad$ positive recurrent
- $\{1,2,\cdots\}\quad \text{ }\text{ }\quad$transient

But the chain does not necessarily end up with being in state $0$, because it can also have $X(t)\rightarrow\infty$. Whether this is a possibility depends on the relation between $\{\lambda_i\}$ and $\{\mu_i\}$.

